therefore implies that $\begin{array} { r } { 1 = \sum _ { v \in \Lambda ^ { 0 } } \sum _ { i = 0 } ^ { n - 1 } S _ { v , w _ { i } } } \end{array}$ . Consequently,

$$
\begin{array} { r l } & { U _ { j } U _ { j } ^ { * } = \left( \displaystyle \sum _ { v \in \Lambda ^ { 0 } } \displaystyle \sum _ { i = 0 } ^ { n - 1 } S _ { ( v , f _ { i , j } ) } ^ { * } \right) \left( \displaystyle \sum _ { u \in \Lambda ^ { 0 } } \displaystyle \sum _ { m = 0 } ^ { n - 1 } S _ { ( u , f _ { m , j } ) } \right) } \\ & { \quad \quad = \displaystyle \sum _ { v \in \Lambda } \displaystyle \sum _ { i = 0 } ^ { n - 1 } S _ { ( v , f _ { i , j } ) } ^ { * } S _ { ( v , f _ { i , j } ) } = \displaystyle \sum _ { v \in \Lambda } \displaystyle \sum _ { i = 0 } ^ { n - 1 } S _ { v , w _ { i } } } \\ & { \quad \quad = 1 = \left( \displaystyle \sum _ { v \in \Lambda ^ { 0 } } \displaystyle \sum _ { i = 0 } ^ { n - 1 } S _ { ( v , f _ { i , j } ) } \right) \left( \displaystyle \sum _ { u \in \Lambda ^ { 0 } } \displaystyle \sum _ { m = 0 } ^ { n - 1 } S _ { ( u , f _ { m , j } ) } ^ { * } \right) } \\ & { \quad \quad = U _ { j } ^ { * } U _ { j } . } \end{array}
$$

We conclude that $\{ U _ { j } \}$ is a unitary representation of $\mathbb { Z } ^ { k _ { 2 } }$ contained in $C ^ { * } ( \Omega )$ .

To see that conjugation by $U _ { j }$ will induce the action of $\rho _ { j }$ , fix $\lambda \in \Omega _ { 1 } ^ { w _ { m } } ( \cong \Lambda )$ . By Lemma 2.9,

$$
( \lambda , w _ { m } ) ( s ( \lambda ) , f _ { m - 1 , j } ) = ( r ( \lambda ) , f _ { m - 1 , j } ) ( ( \widehat { f } _ { m - 1 , j } ) _ { \triangleleft } ( \lambda ) , w _ { m - 1 } )
$$

since $C _ { n , k _ { 2 } }$ is a stable quasi-factor. (CK2) now implies that

$$
\begin{array} { l }  \displaystyle U _ { j } S _ { ( \lambda , w _ { m } ) } U _ { j } ^ { * } = \left( \overset { n - 1 } { \sum _ { i = 0 } ^ { n } \} \sum _ { v \in \Lambda ^ { 0 } } S _ { ( v , f _ { i , j } ) } ^ { * } \right) S _ { ( \lambda , w _ { m } ) } \left( \overset { n - 1 } { \sum _ { \ell = 0 } ^ { n } } \underset { u \in \Lambda ^ { 0 } } { \sum _ { \ell = 1 } ^ { n } \sum } S _ { ( u , f _ { \ell , j } ) } \right) } \\ { \displaystyle \quad \quad = S _ { ( r ( \lambda ) , f _ { m - 1 , j } ) } ^ { * } S _ { ( \lambda , w _ { m } ) } \left( \overset { n - 1 } { \sum _ { \ell = 0 } ^ { n } } \sum _ { u \in \Lambda ^ { 0 } } S _ { ( u , f _ { \ell , j } ) } \right) } \\ { \displaystyle \quad \quad = S _ { ( r ( \lambda ) , f _ { m - 1 , j } ) } ^ { * } S _ { ( \lambda , w _ { m } ) } S _ { ( s ( \lambda ) , f _ { m - 1 , j } ) } } \\ { \displaystyle \quad \quad = S _ { ( r ( \lambda ) , f _ { m - 1 , j } ) } ^ { * } S _ { ( r ( \lambda ) , f _ { m - 1 , j } ) } S _ { ( ( \widehat { f _ { m - 1 , \lambda } } , \widehat { \mathbf { \xi } } ) ) , ( \widehat { \lambda } , w _ { m } ) } } \\ { \displaystyle \quad \quad = S _ { ( ( \widehat { f _ { m - 1 , j } } ) , \widehat { \mathbf { \xi } } ) } ^ { * } ( \lambda ) , w _ { m } ) = { { \widehat { \rho _ { m - 1 , j } } } } \int S _ { ( ( \widehat { f _ { \lambda , w _ { m } } } ) ) } \ d s . } \end{array}
$$

As each $\rho _ { i , j }$ is a $^ *$ -homomorphism, and $C ^ { * } ( \Omega _ { 1 } ^ { w _ { m } } )$ is generated by $\{ S _ { ( \lambda , w _ { m } ) } \} _ { \lambda }$ , we conclude that the automorphism $\rho _ { j }$ of $\bigoplus _ { i = 0 } ^ { n - 1 } C ^ { * } ( \Omega _ { 1 } ^ { w _ { i } } )$ is indeed given by conjugation by $U _ { j }$ .

This demonstrates that $\{ U _ { j } \} _ { j = 1 } ^ { k _ { 2 } }$ yields a unitary representation of $\mathbb { Z } ^ { k _ { 2 } }$ which induces $\rho$ on $C ^ { * } ( \Omega _ { 1 } ) \cong \bigoplus _ { i = 0 } ^ { n - 1 } C ^ { * } ( \Omega _ { 1 } ^ { w _ { i } } )$ via conjugation. The universal property of the crossed product now gives a $^ *$ -homomorphism

$$
\Phi : \left( \bigoplus _ { i = 0 } ^ { n - 1 } C ^ { * } ( \Omega _ { 1 } ^ { w _ { i } } ) \right) \rtimes _ { \rho } \mathbb { Z } ^ { k _ { 2 } } \to C ^ { * } ( \Omega )
$$

with image $\langle C ^ { * } ( \Omega _ { 1 } ) , U _ { j } \rangle$ . It remains to show that $\Phi$ is bijective.

We demonstrate surjectivity by observing first that each vertex projection $S _ { ( v , w _ { i } ) }$ lies in $C ^ { * } ( \Omega _ { 1 } )$ and therefore $S _ { ( v , w _ { i + 1 } ) } U _ { j } ^ { * } = S _ { ( v , f _ { i , j } ) } \in \mathrm { I m } \Phi$ for all $v , i , j$ . In particular, every generator of $C ^ { * } ( \Omega _ { 2 } )$ lies in $\operatorname { I m } \Phi$ , making the image all of $C ^ { * } ( \Omega )$ .

To demonstrate injectivity, we construct a Cuntzâ€“Krieger $\Omega$ -family inside of $( \bigoplus _ { i } C ^ { * } ( \Omega _ { 1 } ^ { w _ { i } } ) ) \ \rtimes _ { \rho } \mathbb { Z } ^ { k _ { 2 } }$ , such that the associated $^ *$ -homomorphism $\Psi : C ^ { * } ( \Omega ) \to$ $( \bigoplus _ { i } C ^ { * } ( \Omega _ { 1 } ^ { w _ { i } } ) ) \rtimes _ { \rho } \mathbb { Z } ^ { k _ { 2 } }$ satisfies $\Psi \Phi = \mathrm { i d }$ . To that end, write $V _ { j }$ for the canonical generators of $\mathbb { Z } ^ { k _ { 2 } }$ in the crossed product, and for each $e \in G ( \Lambda ) ^ { 1 } , f _ { i , j } \in C _ { n , k _ { 2 } } ^ { 1 }$ and each vertex $v \in \Lambda ^ { 0 } , w _ { i } \in C _ { n , k _ { 2 } } ^ { 0 }$ , define $T _ { ( e , w _ { i } ) } , T _ { ( v , w _ { i } ) } , T _ { ( v , f _ { i , j } ) } \in ( \bigoplus _ { i } C ^ { * } ( \Omega _ { 1 } ^ { w _ { i } } ) ) \rtimes _ { \rho } \mathbb { Z } ^ { k _ { 2 } }$