Define $a _ { 0 } : = \infty$ , $\begin{array} { r } { a _ { n } : = \sum _ { k \geq n } \mu _ { + } ^ { - 1 } ( \delta ^ { k } ) / k } \end{array}$ for $n \in \mathbb { N }$ , and the function $\psi$ by

$$
\psi ( t ) : = \ \sum _ { n \in \mathbb { N } _ { 0 } } \delta ^ { n } \mathbb { 1 } _ { ( a _ { n + 1 } , a _ { n } ] } ( t ) , \quad t \geq 0 .
$$

Then

$$
F ( t ) \ \leq \ \psi ( 4 t ) \quad f o r \ a l l \ t \leq t _ { 0 } : = { \frac { \delta } { 4 ( 2 + \delta ) } } \mu _ { + } ^ { - 1 } ( 1 ) .
$$

Proof. The assumptions imply that $\mu _ { + }$ is continuous and strictly increasing and hence is the cumulative mass function of a continuous measure on $[ 0 , \infty )$ . Moreover, $\mu _ { + }$ is a bijection of $[ 0 , \infty )$ , and its generalized inverse $\mu _ { + } ^ { - 1 }$ is simply the inverse function. Let $\psi _ { 0 } = \psi$ , and for $n \in  { \mathbb { N } }$ , define $\psi _ { n }$ recursively by

$$
\psi _ { n + 1 } ( t ) : = 1 - \exp \bigg ( - \psi _ { n } ( t ) - \int _ { 0 } ^ { t / 4 } \psi _ { n } ( t - 4 x ) \mu _ { + } ( \mathrm { d } x ) \bigg ) , \quad t \geq 0 .
$$

Denote by $\mathbf { T }$ denoting the smoothing transform associated with the Poisson point process with intensity measure $\mu = \delta _ { 0 } + \mu _ { + }$ as given by (3.2) and its representation (5.1). By induction, we observe that

$$
1 - \psi _ { n } ( 4 t ) \ = \ \mathbf { T } ^ { n } \left[ 1 - \psi ( 4 ( \cdot ) ) \right] ( t ) , \quad t \geq 0 .
$$

Thus, by Theorem 3.4(b), we infer that $\psi _ { n } ( 4 t )  F ( t )$ as $n \to \infty$ for all $t > 0$ .

To complete the proof, it remains to show that $\psi _ { n } ( t ) \leq \psi ( t )$ holds for all $t \leq 4 t _ { 0 }$ and $n \in  { \mathbb { N } } _ { 0 }$ . We will prove the slightly stronger statement $\psi _ { n } ( t ) \leq \psi ( t )$ for all $t \leq a _ { k _ { 0 } }$ via induction on $n$ , where $\boldsymbol k _ { 0 } \in \mathbb { N } _ { 0 }$ is chosen such that

$$
a _ { k _ { 0 } + 1 } < 4 t _ { 0 } \leq a _ { k _ { 0 } } .
$$

For $n = 0$ , the claim is trivially true (base case). For the inductive step, assume $\psi _ { n } ( t ) \leq \psi ( t )$ for all $t \leq a _ { k _ { 0 } }$ and some $n \in  { \mathbb { N } } _ { 0 }$ . We will show that $\psi _ { n + 1 } ( t ) \leq \psi ( t )$ for all $t \in ( a _ { k + 1 } , a _ { k } ]$ and $k \geq k _ { 0 }$ . If $k _ { 0 } = 0$ , for $t > a _ { 1 }$ we clearly have $\psi ( t ) = 1 \geq \psi _ { n + 1 } ( t )$ . Thus we can assume $k \geq k _ { 0 } \vee 1$ . Let $t \in ( a _ { k + 1 } , a _ { k } ]$ for $k \geq k _ { 0 } \vee 1$ . Then we have

$$
\begin{array} { r c l } { \psi _ { n + 1 } ( t ) \ \leq \ \psi _ { n + 1 } ( a _ { k } ) \ = \ 1 - \exp \bigg ( - \psi _ { n } ( a _ { k } ) - \displaystyle \int _ { 0 } ^ { a _ { k } / 4 } \psi _ { n } ( a _ { k } - 4 x ) \mu _ { + } ( \mathrm { d } x ) \bigg ) } \\ { \displaystyle \leq \ 1 - \exp \bigg ( - \psi ( a _ { k } ) - \displaystyle \int _ { 0 } ^ { a _ { k } / 4 } \psi ( a _ { k } - 4 x ) \mu _ { + } ( \mathrm { d } x ) \bigg ) } \\ { \displaystyle = \ 1 - \exp \big ( - ( \psi ( t ) + I _ { k } ) \big ) } \end{array}
$$

where $I _ { k }$ represents the integral in the exponent. To estimate $I _ { k }$ , we first note that

$$
\begin{array} { r l } { I _ { k } \ = \ \displaystyle \int _ { 0 } ^ { a _ { k } / 4 } \psi ( a _ { k } - 4 x ) \mu _ { + } ( \mathrm { d } x ) \ = \ \displaystyle \sum _ { j \ge k } \int _ { [ a _ { k } - a _ { j } , a _ { k } - a _ { j + 1 } ) / 4 } \psi ( a _ { k } - 4 x ) \mu _ { + } ( \mathrm { d } x ) } \\ { \displaystyle \ = \ \displaystyle \sum _ { j \ge k } \delta ^ { j } \biggl [ \mu _ { + } \Bigl ( \frac { a _ { k } - a _ { j + 1 } } { 4 } \Bigr ) - \mu _ { + } \Bigl ( \frac { a _ { k } - a _ { j } } { 4 } \Bigr ) \biggr ] } \\ { \displaystyle \ = \ \delta ^ { k } \displaystyle \sum _ { j = 0 } ^ { \infty } \delta ^ { j } \biggl [ \mu _ { + } \Bigl ( \frac { a _ { k } - a _ { k + j + 1 } } { 4 } \Bigr ) - \mu _ { + } \Bigl ( \frac { a _ { k } - a _ { k + j } } { 4 } \Bigr ) \biggr ] } \\ { \displaystyle \ = \ \psi ( t ) \displaystyle \sum _ { j = 0 } ^ { \infty } \delta ^ { j } ( 1 - \delta ) \mu _ { + } \Bigl ( \frac { a _ { k } - a _ { k + j + 1 } } { 4 } \Bigr ) , } \end{array}
$$