# 3.3. Global existence.

Theorem 3.10. Assuming that (3.2) and (3.3) are satisfied, then the conclusions in Theorem 3.4 hold for any $T ' > 0$ .

Proof. By Theorem 3.4, we may assume that (3.1) has a unique solution $( u , g , h )$ defined on some maximal time interval $( 0 , T _ { m } )$ with $T _ { m } \in ( 0 , \infty ]$ , and

$$
h , g \in C ^ { 1 + \frac { \beta } { 2 } } ( ( 0 , T _ { m } ) ) , \quad u \in C ^ { 1 + \frac { \beta } { 2 } , 2 + \beta } ( \Omega _ { T _ { m } } ) ,
$$

where $\Omega _ { T _ { m } } : = \{ ( t , x ) : t \in ( 0 , T _ { m } ) , x \in [ g ( t ) , h ( t ) ] \}$ . To complete the proof, we must demonstrate that $I _ { m } ^ { \prime } = \infty$ . Suppose $T _ { m } < \infty$ . Then, by the proof of Theorem 3.4, along with Lemmas 3.8 and 3.9, there exist positive constants $C _ { 1 } , C _ { 2 } = C _ { 2 } ( T _ { m } )$ , such that for $t \in  { \left. 0 , T _ { m } \right. }$ and $x \in [ g ( t ) , h ( t ) ]$ ,

For any small constant $\varepsilon > 0$ , it follows from the proof of Theorem 3.4 and Lemmas 3.8 and 3.9 that $u , v \in C ^ { 1 + \beta , \frac { 1 + \beta } { 2 } } ( \Omega _ { T _ { m } - \varepsilon } )$ . Thus, as in Step 4 of the proof of Theorem 3.4, applying Schauder’s estimates, for any fixed 0 < T0 < Tm − ε, we obtain ∥u∥C2+β,1+ β2 (ΩT −ε\ΩT ) ≤ Q∗, where Q∗ depends on T0, Tm, and $C _ { i }$ for $i = 1 , 2$ , but is independent of $\varepsilon$ . Since $\varepsilon > 0$ can be made arbitrarily small, it follows that for any $t \in [ T _ { 0 } , T _ { m } )$ ,

$$
\| u ( t , \cdot ) \| _ { C ^ { 2 + \beta } ( [ g ( t ) , h ( t ) ] ) } \leq Q ^ { * }
$$

By repeating the arguments used in the proof of Theorem 3.4, we can conclude that there exists $T > 0$ small, depending on $Q ^ { * }$ and $C _ { i }$ ( $i = 1 , 2$ ), such that the solution to (3.1) with initial time $T _ { m } - { \frac { \pi } { 2 } }$ can be extended uniquely to $\begin{array} { r } { t = T _ { m } - \frac { T } { 2 } + T > T _ { m } } \end{array}$ , a contradiction to the definition that $x _ { m }$ is the maximal time interval for the solution. Thus, we must have $T _ { m } = \infty$ . □

3.4. Proof of Theorem 3.1. Let us first note that $f ( t , x , 1 ) \equiv 0$ and $f ( t , x , u ) \leq f ( u ) < 0$ for $u > 1$ imply $f ( 1 ) = 0$ . Let $M _ { 0 } = \operatorname* { m a x } \{ \| u _ { 0 } \| _ { \infty } , 1 \}$ and $v ( t )$ be the solution of

$$
v ^ { \prime } = \bar { f } ( v ) , \ v ( 0 ) = M _ { 0 } .
$$

Since $f ( v ) < 0$ for $v > 1$ , we clearly have $1 \leq v ( t ) \leq M _ { 0 }$ and $v ( t ) \to 1$ as $t \to \infty$ . Since $f ( t , x , u ) \leq f ( u )$ for $u \geq 1$ , we obtain

We also have $v \geq 1 > \delta = u$ for $x \in \{ g ( t ) , h ( t ) \}$ and $v ( 0 ) = M _ { 0 } \geq u ( 0 , x )$ for $x \in [ - h _ { 0 } , h _ { 0 } ]$ . Therefore the standard comparison principle over the region $\{ ( t , x ) : t > 0 , x \in [ g ( t ) , h ( t ) ] \}$ infers $u ( t , x ) \leq v ( t )$ in this region. It follows that

$$
\operatorname* { l i m } _ { t \to \infty } u ( t , x ) \leq \operatorname* { l i m } _ { t \to \infty } v ( t ) = 1
$$

To bound $u ( t , x )$ from below, we first make use of (3.4) to show that there exists $T _ { 0 } > 0$ such that (3.32) $u ( t , x ) \geq \delta$ for $t \geq T _ { 0 }$ and $x \in [ g ( t ) , h ( t ) ]$ .

Similar to the proof of Theorem 1.1, since $\underline { { f } }$ satisfies ( $\mathbf { f _ { A } }$ ), we are able to choose a function $\hat { f } \in C ^ { 1 }$ sufficiently close to $\underline { { f } }$ in $L ^ { \infty }$ such that ${ \hat { f } } ( s ) \leq f ( s )$ for $s \geq 0$ , and $\hat { f }$ satisfies $\left( \mathbf { F _ { b } } \right)$ with $( P , Q ) = ( { \hat { \theta } } , \delta )$ for some $\hat { \theta } \in [ \theta , \delta ) \cap ( 0 , \delta )$ . Then, by Lemma 2.1, the traveling wave problem (2.4) has a solution pair $( c , q ) = ( c _ { 0 } , q _ { 0 } )$ with $c _ { 0 } > 0$ and $q _ { 0 } ( \cdot )$ strictly increasing.

The same reasoning as in the proof of Theorem 1.1 shows that for some $L > 0$ sufficiently large,

$$
\underline { { u } } ( t , x ) : = \operatorname* { m a x } \{ q _ { 0 } ( c t - x - L ) , q _ { 0 } ( c t + x - L ) \}
$$

satisfies (in the weak sense)

$$
u _ { t } \leq d \underline { { u } } _ { x x } + \underline { { f } } ( \underline { { u } } ) \leq f ( t , x , \underline { { u } } ) \quad \mathrm { f o r ~ } t > 0 , \ x \in \mathbb { R } .
$$

Additionally,

$$
0 \leq \underline { { u } } ( t , x ) \leq \delta \leq u ( t , x ) \mathrm { ~ f o r ~ } t > 0 , \ x \in \{ g ( t ) , h ( t ) \} ,
$$

and

$$
\underline { { u } } ( 0 , x ) \leq u _ { 0 } ( x ) \quad \mathrm { f o r } ~ x \in [ - h _ { 0 } , h _ { 0 } ]
$$

Therefore we can apply the standard comparison principle over $\{ ( t , x ) : t > 0 , x \in [ g ( t ) , h ( t ) ] \}$ to deduce $u ( t , x ) \geq \underline { { u } } ( t , x )$ in this region.

Moreover, using

$$
\operatorname* { l i m } _ { t \to \infty } \| \underline { { u } } ( t , \cdot ) - \delta \| _ { L ^ { \infty } ( \mathbb { R } ) } = 0 ,
$$