which converges in  $\mathcal{O}^{L\text{-la}}_{\mathcal{M}_{\mathrm{LT},\infty}}(U)$ . Later we will show  $D_i(s)$  acturally lies in the smaller subspace  $\mathcal{O}^{L\text{-la},\mathfrak{m}^0=0}_{\mathcal{M}_{\mathrm{LT},\infty}}(U)$ . Using  $E_{d,i}(x_i - x_{i,n}) = 1$ , a direct computation shows  $E_{d,i}.D_i(s) = 0$  for all  $s \in \mathcal{O}_{\mathcal{M}_{\mathrm{LT},\infty}}^{L\text{-la},\mathfrak{m}^0=0}(U)$ , and

$$s = \sum_{l=0}^{\infty} a_{i,l} (x_i - x_{i,n})^l$$

with  $a_{i,l} = D_i(\frac{(E_{d,i})^l.s}{l!})$ . Here we note the coefficients  $a_{i,l}$  are determined by s. From the construction we know the coefficients  $a_{i,l}$  are killed by  $E_{d,i}$  for all l. For  $j \neq i$ , we furthure express the coefficients  $a_{i,l}$  along  $E_{d,i}$ , namely

$$a_{i,l} = \sum_{k=0}^{\infty} b_{i,l,j,l'} (x_j - x_{j,n})^{l'}$$

with  $b_{i,l,j,l'} = D_j(\frac{(E_{d,j})^{l'} \cdot a_{i,l}}{l'!})$ . As  $[E_{d,i}, E_{d,j}] = 0$  for  $i, j = 0, 1, ..., d-1$ , we see  $b_{i,l,j,l'}$  is killed by  $E_{d,i}$  and  $E_{d,j}$ . After we expand s along each derivation  $E_{d,i}$  for  $i = 0, 1, ..., d-1$ , we arrive at an exp

$$s = \sum_{i_0=0}^{\infty} \sum_{i_1=0}^{\infty} \cdots \sum_{i_{d-1}=0}^{\infty} c_{i_0 \dots i_{d-1}} (x_0 - x_{0,n})^{i_0} \cdots (x_{d-1} - x_{d-1,n})^{i_{d-1}}$$

such that  $E_{d,i}c_{i_0...i_{d-1}} = 0$  for all  $i = 0, 1, ..., d-1$ . As  $\mathfrak{m}^0$  acts trivially on  $\mathcal{O}_{\mathscr{F}\ell}$ , we know  $\mathfrak{m}^0$  acts trivially on  $x_i - x_{i,n}$  for any  $i = 0, ..., d-1$ . Therefore,

$$0 = \sum_{i_0,\ldots,i_{d-1}} (\mathfrak{m}^0 c_{i_0\ldots i_{d-1}}) (x_0 - x_{0,n})^{i_0} \cdots (x_{d-1} - x_{d-1,n})^{i_{d-1}}$$

This implies  $\mathfrak{m}^0 c_{i_0 \dots i_{d-1}} = 0$ . Indeed, the coefficients  $c_{i_0 \dots i_{d-1}}$  are determined by s. Combined this with the fact that  $\mathcal{O}_{\mathcal{M}_{\mathrm{LT},\infty}}^{L\text{-la}}$  is killed by  $\pi^{-1}\mathfrak{n}^0$ , we see  $\mathfrak{p}^0$  kills  $c_{i_0...i_{d-1}}$ . Hence there is an induced action of  $\overline{\mathfrak{n}}^0 = \mathfrak{g}^0/\mathfrak{p}^0$ on  $c_{i_0...i_{d-1}}$ . On  $U$ ,  $\overline{\mathfrak{n}}^0$  is generated by  $E_{d,i}$  for  $i = 0, 1, ..., d-1$ . Indeed, on the open locus  $V_o = \{[z_0 : z_1 : \cdots : z_{d-1} : 1]\} \subset \mathbb{P}^d$ , the matrix  $Z = \begin{pmatrix} I_{d \times d} & 0 \\ (z_0, z_1, ..., z_{d-1}) & 1 \end{pmatrix}$  is a lift as  $oZ = z$  where  $o = [0:0:\cdots:0:1]$ . Then  $Z^{-1}E_{d,i}Z = E_{d,i}$  for  $i = 0,1,...,d$  generates  $\overline{\mathfrak{n}}^0$  on  $V_o$ . From the construction we know  $c_{i_0...i_{d-1}}$  is killed by  $E_{d,i}$  for all  $i = 0, 1, ..., d-1$ , hence it is killed by  $\overline{\mathfrak{n}}^0$ . This shows that  $\mathfrak{g}^0$  acts trivally on  $c_{i_0...i_{d-1}}$ , which implies  $c_{i_0...i_{d-1}} \in \mathcal{O}_{\mathcal{M}_{\mathrm{LT},\infty}}^{\mathrm{sm}}(U)$ . ÐŸ

Corollary 0.3.2. For any  $U \in \mathfrak{B}_{\mathrm{LT}}$ , the image of  $\mathcal{O}_{\mathcal{M}_{\mathrm{LT},\infty}}^{\mathrm{sm}}(U) \otimes_C \pi^{-1}\mathcal{O}_{\mathscr{F}\ell}(U)$  inside  $\mathcal{O}_{\mathcal{M}_{\mathrm{LT},\infty}}^{L\text{-la},\mathfrak{m}^0=0}(U)$  is dense.  $Proof.$  This follows directly from Theorem 0.3.1.  $\Box$ 

To simplify the notation, we denote  $\mathcal{O}_{\mathrm{LT}}$  by the sheaf  $\mathcal{O}_{\mathcal{M}_{\mathrm{LT},\infty}}^{L\text{-la},\mathfrak{m}^0=0}$  on  $\mathcal{M}_{\mathrm{LT},\infty}$ . Put  $\mathcal{O}_{\mathrm{LT}}^{\mathrm{sm}} := \mathcal{O}_{\mathcal{M}_{\mathrm{LT},\infty}}^{G\text{-sm}}$ . Let  $\Omega_{\mathcal{M}_{\mathrm{LT},n}}^k$  be the sheaf o

**Proposition 0.3.3.** There exists a differential operator  $d: \mathcal{O}_{\mathrm{LT}} \to \mathcal{O}_{\mathrm{LT}} \otimes_{\mathcal{O}_{\mathrm{LT}}} \Omega_{\mathrm{LT}}^{1,\mathrm{sm}}$ , such that

- (i) d is given by the usual derivation on  $\mathcal{O}_{\text{LT}}^{\text{sm}}$ ,
- (ii)  $d$  is  $\pi^{-1}\mathcal{O}_{\mathscr{F}\ell}$ -linear.

Moreover,  $d$  is uniquely determined by these two properties up to constants.

*Proof.* Define  $d|_{\mathcal{O}^{\text{sm}}_{\text{LT}}}$  as the differential map on finite levels  $\mathcal{O}^{\text{sm}}_{\text{LT}} \to \Omega^{1,\text{sm}}_{\text{LT}}$ , and define  $d|_{\pi^{-1}\mathcal{O}_{\mathscr{F}\ell}}$  to be the zero map. By Theorem 0.3.1, for any  $U \in \mathfrak{B}_{\mathrm{LT}}$  such that  $z_d \neq 0$  on U, we may write any section  $s \in \mathcal{O}_{\mathrm{LT}}(U)$  of the form for some sufficiently large  $n$ :

$$s = \sum_{i_0=0}^{\infty} \sum_{i_1=0}^{\infty} \cdots \sum_{i_{d-1}=0}^{\infty} c_{i_0 \dots i_{d-1}} (x_0 - x_{0,n})^{i_0} \cdots (x_{d-1} - x_{d-1,n})^{i_{d-1}}$$