Note that one can choose any  $\vec{\Theta}$  satisfying

$$\max\{-1, -1 - v_p(x_1)\} \le v_p(\Theta_0) = 1 - v_p(\Theta_1) \le \min\{0, v_p(x_0)\}.$$

We will divide  $R(\vec{r}; \vec{k}')$  into following four areas, and in each area we will determine the  $\text{mod-}p$  reduction:

- (i)  $\vec{t} \in R_{int}(\vec{r}; \vec{k}')$ : Note that we have either  $v_p(\Theta_0) \notin \{0, v_p(x_0)\}$  or  $v_p(\Theta_0) \notin \{0, v_p(x_0)\}$  $\{-1, -1 - v_p(x_1)\}\text{, in this case. Consider two } \overline{S}_{\mathbf{F}}\text{-submodules } \mathcal{M}' = \overline{S}_{\mathbf{F}}(\overline{E}_1^{(0)}, \overline{E}_2^{(1)})$ and  $\mathcal{M}'' = \overline{S}_{\mathbf{F}}(\overline{E}_2^{(0)}, \overline{E}_1^{(1)})$  of  $\mathcal{M}$ . Then one can observe that
  - $\circ$  if  $v_p(\Theta_0) \notin \{0, v_p(x_0)\},$  then  $\mathcal{M}'$  is a Breuil submodule of  $\mathcal{M}$  such that  $\mathcal{M}' \cong \mathcal{M}(1,1;-\beta_0,\alpha_1) \text{ and } \mathcal{M}/\mathcal{M}' \cong \mathcal{M}(1,1;\alpha_0,-\beta_1);$
  - $\circ$  if  $v_p(\Theta_0) \notin \{-1, -1 v_p(x_1)\}$ , then  $\mathcal{M}''$  is a Breuil submodule of  $\mathcal{M}$  such that  $\mathcal{M}'' \cong \mathcal{M}(1,1;\alpha_0,-\beta_1)$  and  $\mathcal{M}/\mathcal{M}'' \cong \mathcal{M}(1,1;-\beta_0,\alpha_1)$ .

In particular, if  $v_p(\Theta_0) \notin \{-1, 0, v_p(x_0), -1 - v_p(x_1)\}$ , then  $\mathcal{M} = \mathcal{M}' \oplus \mathcal{M}''$  as Breuil modules. Otherwise, It is not difficult to show that the short exact sequence determined by  $\mathcal{M}' \hookrightarrow \mathcal{M}$  or  $\mathcal{M}'' \hookrightarrow \mathcal{M}$  is non-split. So,  $\overline{\rho}^{ss}|_{I_{\mathbf{Q}_{n^2}}} \cong \omega_2^{p+1} \oplus \omega_2^{p+1}$ ,

by Lemma  $2.3.6$  (i). Furthermore, the monodromy type is given as follow.

- (a) If  $v_p(\Theta_0) = 0$ , then  $t_0 \ge 0$ , and the monodromy type is  $(1,0)$ .
- (b) If  $v_p(\Theta_0) = -1$ , then  $t_1 \ge 0$ , and the monodromy type is  $(0,1)$ .
- (c) Otherwise, the monodromy type is  $(0,0)$ .

(ii)  $t_1 = -1, t_0 \ge 0$ : We have  $v_p(\Theta_0) = 0 = -1 - v_p(x_1)$ , and so  $\frac{1}{\Theta_0}, \frac{x_1}{\Theta_1} \in \mathbf{F}^{\times}$  and  $\frac{1}{\Theta_1} =$ 0 in **F**. In particular, the monodromy type is (1,0). Put  $\mathcal{M}' = \overline{S}_{\mathbf{F}}(\overline{E}_2^{(0)}, \overline{E}_1^{(1)})$ . It is easy to see that  $\mathcal{M}' \cong \mathcal{M}(1,2;\alpha_0, -px_1\beta_1)$  and  $\mathcal{M}/\mathcal{M}' \cong \mathcal{M}(1,0; -\beta_0, \frac{\alpha_1}{px_1}),$ and so we conclude that  $\overline{\rho}^{ss}|_{I_{\mathbf{Q}_{p^2}}} \cong \omega_2^p \oplus \omega_2^{p+2}$ , by Lemma 2.3.6 (i), and  $\overline{\rho}$  is non-split as the monodromy type is nonzero.

(iii)  $t_0 + t_1 = -1, -1 < t_0 < 0$ : We have  $v_p(\Theta_0) = v_p(x_0) = -1 - v_p(x_1) \notin \{-1, 0\},\$ and so  $\frac{x_0}{\Theta_0}, \frac{x_1}{\Theta_1} \in \mathbf{F}^{\times}$  and  $\frac{1}{\Theta_0} = \frac{1}{\Theta_1} = 0$  in **F**. In particular, the monodromy type is  $(0,0)$ . Put

$$A := \begin{bmatrix} -\frac{x_1}{\Theta_1} \alpha_1 & \alpha_1\\ -\beta_1 & 0 \end{bmatrix} \begin{bmatrix} -\frac{x_0}{\Theta_0} \alpha_0 & \alpha_0\\ -\beta_0 & 0 \end{bmatrix} = \begin{bmatrix} \frac{x_0 x_1}{\Theta_0 \Theta_1} \alpha_0 \alpha_1 & -\beta_0 \alpha_1 & -\frac{x_1}{\Theta_1} \alpha_0 \alpha_1\\ \frac{x_0}{\Theta_0} \alpha_0 \beta_1 & -\alpha_0 \beta_1 \end{bmatrix}.$$

Under the base change

$$\underline{E}'^{(1)} = \underline{E}^{(1)} \begin{bmatrix} 0 & -\frac{1}{\beta_1} \\ \frac{1}{\alpha_1} & -\frac{x_1}{\beta_1 \Theta_1} \end{bmatrix}, \ \underline{F}'^{(0)} = \underline{F}^{(0)} \begin{bmatrix} 1 & 0 \\ -\frac{x_0}{\Theta_0} & 1 \end{bmatrix}, \ \underline{F}'^{(1)} = \underline{F}^{(1)} \begin{bmatrix} 0 & -\frac{1}{\beta_1} \\ \frac{1}{\alpha_1} & 0 \end{bmatrix},$$

we have

 $\circ \ \text{Mat}_{\underline{E}^{(0)},\underline{F}'^{(0)}}(\text{Fil}^r\mathcal{M}^{(0)}) = \text{Mat}_{E'^{(1)},F'^{(1)}}(\text{Fil}^r\mathcal{M}^{(1)}) = uI_2;$ 

 $\circ \operatorname{Mat}_{\underline{E}'^{(1)},\underline{F}'^{(0)}}(\phi_2^{(0)}) = A \quad \& \quad \operatorname{Mat}_{\underline{E}^{(0)},\underline{F}'^{(1)}}(\phi_2^{(1)}) = I_2.$ <br>Note that we have  $\frac{\alpha_0}{\beta_0} = \frac{\alpha_1}{\beta_1} = p\Theta_0\Theta_1$  and  $\alpha_0\alpha_1 = \lambda^2\Theta_0\Theta_1$ , and so one can describe the mod-*p* reduction as follo

âˆ˜ if  $px_0x_1 \neq 4$  in **F**, then *A* is diagonalizable. So, extending **F** large enough, we have  $\overline{\rho}|_{I_{\mathbf{Q}_{p^2}}} \cong \omega_2^{p+1} \oplus \omega_2^{p+1}$  by Lemma 2.3.6 (i).