therefore implies that  $1 = \sum_{v \in \Lambda^0} \sum_{i=0}^{n-1} S_{v,w_i}$ . Consequently,

$$\begin{split} U_j U_j^* &= \left(\sum_{v \in \Lambda^0} \sum_{i=0}^{n-1} S^*_{(v, f_{i,j})}\right) \left(\sum_{u \in \Lambda^0} \sum_{m=0}^{n-1} S_{(u, f_{m,j})}\right) \\ &= \sum_{v \in \Lambda} \sum_{i=0}^{n-1} S^*_{(v, f_{i,j})} S_{(v, f_{i,j})} = \sum_{v \in \Lambda} \sum_{i=0}^{n-1} S_{v, w_i} \\ &= 1 = \left(\sum_{v \in \Lambda^0} \sum_{i=0}^{n-1} S_{(v, f_{i,j})}\right) \left(\sum_{u \in \Lambda^0} \sum_{m=0}^{n-1} S^*_{(u, f_{m,j})}\right) \\ &= U^*_j U_j. \end{split}$$

We conclude that  $\{U_j\}$  is a unitary representation of  $\mathbb{Z}^{k_2}$  contained in  $C^*(\Omega)$ .

To see that conjugation by  $U_i$  will induce the action of  $\rho_i$ , fix  $\lambda \in \Omega_1^{w_m} (\cong \Lambda)$ . By Lemma  $2.9$ ,

$$(\lambda, w_m)(s(\lambda), f_{m-1,j}) = (r(\lambda), f_{m-1,j})((\widehat{f}_{m-1,j})_{\triangleleft}(\lambda), w_{m-1})$$

since  $C_{n,k_2}$  is a stable quasi-factor. (CK2) now implies that

$$U_{j}S_{(\lambda,w_{m})}U_{j}^{*} = \left(\sum_{i=0}^{n-1} \sum_{v \in \Lambda^{0}} S_{(v,f_{i,j})}^{*}\right) S_{(\lambda,w_{m})} \left(\sum_{\ell=0}^{n-1} \sum_{u \in \Lambda^{0}} S_{(u,f_{\ell,j})}\right)$$
$$= S_{(r(\lambda),f_{m-1,j})}^{*}S_{(\lambda,w_{m})} \left(\sum_{\ell=0}^{n-1} \sum_{u \in \Lambda^{0}} S_{(u,f_{\ell,j})}\right)$$
$$= S_{(r(\lambda),f_{m-1,j})}^{*}S_{(\lambda,w_{m})}S_{(s(\lambda),f_{m-1,j})}$$
$$= S_{(r(\lambda),f_{m-1,j})}^{*}S_{(r(\lambda),f_{m-1,j})}S_{((\widehat{f}_{m-1,j})_{\lhd}(\lambda),w_{m})}$$
$$= S_{((\widehat{f}_{m-1,j})_{\lhd}(\lambda),w_{m})} = \rho_{m-1,j}(S_{(\lambda,w_{m})}).$$

As each  $\rho_{i,j}$  is a \*-homomorphism, and  $C^*(\Omega_1^{w_m})$  is generated by  $\{S_{(\lambda,w_m)}\}_{\lambda}$ , we conclude that the automorphism  $\rho_j$  of  $\bigoplus_{i=0}^{n-1} C^*(\Omega_1^{w_i})$  is indeed given by conjugation by  $U_j$ .

This demonstrates that  $\{U_j\}_{j=1}^{k_2}$  yields a unitary representation of  $\mathbb{Z}^{k_2}$  which induces  $\rho$  on  $C^*(\Omega_1) \cong \bigoplus_{i=0}^{n-1} C^*(\Omega_1^{w_i})$  via conjugation. The universal property of the crossed product now gives a  $*$ -homomorphism

$$\Phi: \left(\bigoplus_{i=0}^{n-1} C^*(\Omega_1^{w_i})\right) \rtimes_{\rho} \mathbb{Z}^{k_2} \to C^*(\Omega)$$

with image  $\langle C^*(\Omega_1), U_i \rangle$ . It remains to show that  $\Phi$  is bijective.

We demonstrate surjectivity by observing first that each vertex projection  $S_{(v,w_i)}$ lies in  $C^*(\Omega_1)$  and therefore  $S_{(v,w_{i+1})}U_j^* = S_{(v,f_{i,j})} \in \text{Im }\Phi$  for all  $v,i,j$ . In particular, every generator of  $C^*(\Omega_2)$  lies in Im  $\Phi$ , making the image all of  $C^*(\Omega)$ .

To demonstrate injectivity, we construct a Cuntz-Krieger  $\Omega$ -family inside of  $(\bigoplus_i C^*(\Omega_1^{w_i})) \rtimes_{\rho} \mathbb{Z}^{k_2}$ , such that the associated \*-homomorphism  $\Psi : C^*(\Omega) \to$  $\begin{array}{l} (\bigoplus_i C^*(\Omega_1^{w_i})) \rtimes_{\rho} \mathbb{Z}^{k_2} \text{ satisfies } \Psi \Phi = \text{id.} \text{ To that end, write } V_j \text{ for the canonical generators of } \mathbb{Z}^{k_2} \text{ in the crossed product, and for each } e \in G(\Lambda)^1, f_{i,j} \in C^1_{n,k_2} \text{ and each vertex } v \in \Lambda^0, w_i \in C^0_{n,k_2}, \text{define } T_{(e,w_i)}, T_{(v,w_i)}, T_{(v,f_{i,j})} \in (\bigoplus_i C^*(\Omega_1^{w_i})) \rtimes_{\rho} \mathbb{Z}^{k_2} \end{$