**Theorem 3.6.** Let  $\mathbf{x} \preceq (0, \ldots, n-1)$  be an irreducible score, so that  $C \cap (0, \infty)^{n \times n} \neq \emptyset$ .  $Then$ 

$$\lim_{k \to \infty} M^k = \arg\min_{L \in C} D(L, M^0) = \arg\min_{L \in C} H(L). \tag{3.9}$$

*Proof.* Note that dom $(h) = \mathbb{R}_+$ , idom $(h) = (0, \infty)$  and bdom $(h) = \{0\}$ . It is easy to check:

- (1) h is a proper convex function. Moreover, h is closed because  $\{x \in \text{dom}(h) : h(x) \leq \alpha\}$ is closed for all  $\alpha \in \mathbb{R}$ .
- $(2)$  h is Legendre because
  - $h$  is differentiable on  $\text{idom}(h)$ ;
  - $\lim_{t\to 0+} h'(x+t(y-x))(y-x) = -\infty$  for all  $x\in \text{bdom}(f)$  and  $y\in \text{idom}(h)$ ;
  - $h$  is strictly convex on  $\text{idom}(h)$ .
- (3) *h* is co-finite because  $\lim_{t\to\infty}\frac{h(tx)}{t}=\infty$  for all  $x\neq 0$ .
- (4) h is very strictly convex because  $h''(x) > 0$  for all  $x \in \text{idom}(h)$ .

Since  $C_1, C_2, C_3$  are all affine subsets, it suffices to apply [7, Theorem 4.3] to conclude.  $\Box$ 

See also  $[45]$  for recent development on the convergence rate of Bregman's iteration under further technical assumptions, which we do not pursue here.

Next we propose a computational scheme inspired by Theorem 3.6. The key is to compute numerically, for each  $M \in (0,\infty)^{n \times n}$ , its Bregman projection on  $C_k$ . We distinguish three  $cases:$ 

•  $k = 1$ : We introduce the Lagrange multiplier  $\lambda = (\lambda_1, \ldots, \lambda_n) \in \mathbb{R}^n$ , and set  $\n\Phi(L,\lambda) := D(L,M) + \sum_{i=1}^{n} \lambda_i \left( \sum_{j=1}^{n} l_{ij} - 1 \right).\n$ Differentiating  $\Phi$  with respect to  $m_{ij}$  and  $\lambda_i$  yields  $\partial_{l_{ij}} \Phi = \log(l_{ij}) - \log(m_{ij}) + \lambda_i$  and  $\partial_{\lambda_i} \Phi = \sum_{j=1}^{n} l_{ij} - 1$ . By setting these to zero, we get

$$\arg\min_{L \in C_1} D(L, M) = \left(\frac{m_{ij}}{\sum_{k=1}^n m_{ik}}\right)_{1 \le i, j \le n}.\tag{3.10}$$

•  $k = 2$ : The same reasoning as in the previous case yields:

$$\arg\min_{L \in C_2} D(L, M) = \left(\frac{m_{ij}}{\sum_{k=1}^n m_{kj}}\right)_{1 \le i, j \le n}.\tag{3.11}$$

•  $k = 3$ : Define  $\Phi(L, \lambda) := D(L, M) + \sum_{i=1}^{n} \lambda_i \left( \sum_{j=1}^{n} (j-1) l_{ij} - x_i \right)$ , and differentiate  $\Phi$  with respect to  $m_{ij}$  and  $\lambda_i$  yields  $\partial_{l_{ij}}\Phi = \log(l_{ij}) - \log(m_{ij}) + \lambda_i(j-1)$  and  $\partial_{\lambda_i} \Phi = \sum_{j=1}^n (j-1) l_{ij} - x_i$ . Setting these to zero yields

$$\arg\min_{L\in C_3} D(L,M) = \left(m_{ij}r_{ij}^{j-1}\right)_{1\le i,j\le n},\tag{3.12}$$

where  $r_{ij}$  is the unique positive root to the polynomial equation  $\sum_{j=1}^{n} (j-1)m_{ij}r^{j-1} - x_i = 0$ . Let  $f(r) := \sum_{j=1}^{n} (j-1)m_{ij}r^{j-1} - x_i$ . It is easy to see that  $f$  is strictly increasing on  $[0,\infty)$  with  $f(0) \leq 0$  and  $\lim_{r \to \infty} f(r) = +\infty$ . Thus, it is easy (and quick) to find a numerical root of  $f$  on  $[0,\infty)$  by Newton's method.