Define  $a_0 := \infty$ ,  $a_n := \sum_{k>n} \mu_+^{-1}(\delta^k)/k$  for  $n \in \mathbb{N}$ , and the function  $\psi$  by

$$\psi(t) \coloneqq \sum_{n \in \mathbb{N}_0} \delta^n \mathbb{1}_{(a_{n+1}, a_n]}(t), \quad t \ge 0.$$

 $Then$ 

$$F(t) \leq \psi(4t) \quad \text{for all } t \leq t_0 := \frac{\delta}{4(2+\delta)} \mu_+^{-1}(1).$$

*Proof.* The assumptions imply that  $\mu_{+}$  is continuous and strictly increasing and hence is the cumulative mass function of a continuous measure on  $[0,\infty)$ . Moreover,  $\mu_+$  is a bijection of  $[0,\infty)$ , and its generalized inverse  $\mu_+^{-1}$  is simply the inverse function. Let  $\psi_0 = \psi$ , and for  $n \in \mathbb{N}$ , define  $\psi_n$  recursively by

$$\psi_{n+1}(t) := 1 - \exp\bigg(-\psi_n(t) - \int_0^{t/4} \psi_n(t - 4x) \,\mu_+(\mathrm{d}x)\bigg), \quad t \ge 0$$

Denote by  $\mathbf{T}$  denoting the smoothing transform associated with the Poisson point process with intensity measure  $\mu = \delta_0 + \mu_+$  as given by (3.2) and its representation (5.1). By induction, we observe that

$$1 - \psi_n(4t) = \mathbf{T}^n \left[ 1 - \psi(4(\cdot)) \right](t), \quad t \ge 0.$$

Thus, by Theorem 3.4(b), we infer that  $\psi_n(4t) \to F(t)$  as  $n \to \infty$  for all  $t > 0$ .

To complete the proof, it remains to show that  $\psi_n(t) \leq \psi(t)$  holds for all  $t \leq 4t_0$  and  $n \in \mathbb{N}_0$ . We will prove the slightly stronger statement  $\psi_n(t) \leq \psi(t)$  for all  $t \leq a_{k_0}$  via induction on n, where  $k_0 \in \mathbb{N}_0$  is chosen such that

$$a_{k_0+1} < 4t_0 \le a_{k_0}.\tag{5.3}$$

For  $n = 0$ , the claim is trivially true (base case). For the inductive step, assume  $\psi_n(t) \leq \psi(t)$  for all  $t \le a_{k_0}$  and some  $n \in \mathbb{N}_0$ . We will show that  $\psi_{n+1}(t) \le \psi(t)$  for all  $t \in (a_{k+1}, a_k]$  and  $k \ge k_0$ .<br>If  $k_0 = 0$ , for  $t > a_1$  we clearly have  $\psi(t) = 1 \ge \psi_{n+1}(t)$ . Thus we can assume  $k \ge k_0 \vee 1$ . Let  $t \in (a_{k+1}, a_k]$  for  $k \geq k_0 \vee 1$ . Then we have

$$\psi_{n+1}(t) \leq \psi_{n+1}(a_k) = 1 - \exp\left(-\psi_n(a_k) - \int_0^{a_k/4} \psi_n(a_k - 4x) \mu_+(dx)\right)$$
  
$$\leq 1 - \exp\left(-\psi(a_k) - \int_0^{a_k/4} \psi(a_k - 4x) \mu_+(dx)\right)$$
  
$$= 1 - \exp\left(-\left(\psi(t) + I_k\right)\right)$$

where  $I_k$  represents the integral in the exponent. To estimate  $I_k$ , we first note that

$$I_{k} = \int_{0}^{a_{k}/4} \psi(a_{k} - 4x) \mu_{+}(\mathrm{d}x) = \sum_{j \geq k} \int_{[a_{k} - a_{j}, a_{k} - a_{j+1})/4} \psi(a_{k} - 4x) \mu_{+}(\mathrm{d}x)$$
$$= \sum_{j \geq k} \delta^{j} \left[ \mu_{+} \left( \frac{a_{k} - a_{j+1}}{4} \right) - \mu_{+} \left( \frac{a_{k} - a_{j}}{4} \right) \right]$$
$$= \delta^{k} \sum_{j=0}^{\infty} \delta^{j} \left[ \mu_{+} \left( \frac{a_{k} - a_{k+j+1}}{4} \right) - \mu_{+} \left( \frac{a_{k} - a_{k+j}}{4} \right) \right]$$
$$= \psi(t) \sum_{j=0}^{\infty} \delta^{j} (1 - \delta) \mu_{+} \left( \frac{a_{k} - a_{k+j+1}}{4} \right),$$

14