Notice that  $n_i = n_i^1 \wedge n_i^2$ . Thus,

$$\bigwedge_{i=1}^2 n_i = \bigwedge_{i=1}^2 (n_i^1 \wedge n_i^2).$$

Since  $(a_1 \land a_2) \land n_i \neq 0$  for each *i*, we get

$$0 \neq (a_1 \wedge a_2) \wedge n_i = (a_1 \wedge a_2) \wedge (n_i^1 \wedge n_i^2) = (a_1 \wedge n_i^1) \wedge (a_2 \wedge n_i^2).$$

This implies that  $a_1 \wedge n_i^1 \neq 0$  and  $a_2 \wedge n_i^2 \neq 0$ . Since  $a_1 \sim_{\mu} b_1^{\downarrow}$  and  $a_2 \sim_{\mu} b_2^{\downarrow}$ , we have

$$a_1 \wedge \left(\bigwedge_{i=1}^2 n_i^1\right) \neq 0 \quad \text{and} \quad a_2 \wedge \left(\bigwedge_{i=1}^2 n_i^2\right) \neq 0.$$

Thus,

$$(a_1 \wedge a_2) \wedge \left(\bigwedge_{i=1}^2 n_i\right) = (a_1 \wedge a_2) \wedge \left(\bigwedge_{i=1}^2 (n_i^1 \wedge n_i^2)\right) \neq 0.$$

Therefore,  $(a_1 \wedge a_2) \sim_{\mathfrak{u}} (b_1 \wedge b_2)^{\downarrow}$ .

(3) Let  $x_1$  and  $x_2$  be nonzero elements in  $b^{\downarrow}$  such that  $x_1 \wedge x_2 \neq 0$  and  $(a \wedge b) \wedge x_k \neq 0$  for each *k*. This implies  $a \wedge (b \wedge x_k) \neq 0$  for each k. Also, observe that  $\bigwedge_{k=1}^2 (b \wedge x_k) = b \wedge (x_1 \wedge x_2) = x_1 \wedge x_2 \neq 0$ . Since a is a  $\mu$ -element in L, this implies that

$$(a \wedge b) \wedge (x_1 \wedge x_2) = a \wedge \left(\bigwedge_{k=1}^2 (b \wedge x_k)\right) \neq 0,$$

proving the desired claim.

(4) We can assume  $a \ne 0$  and  $a \ne 1$ , because otherwise  $b = 1$  or  $b = 0$  respectively, and the thesis holds. We can also assume that  $c \nleq b$ , because otherwise  $b \vee c = b \rightsquigarrow_{\mathfrak{U}} b^{\uparrow}$ . Let  $x_1 > b$  and  $x_2 > b$  such that  $(x_1 \wedge x_2) > b$  and  $((b \vee c) \wedge x_k) > b$ , for each k. The latter condition is equivalent to  $b \vee (c \wedge x_k) > b$ , which is equivalent to  $c \wedge x_k \nleq b$ . We need to show that

$$(b\vee c)\wedge x_1\wedge x_2>b,$$

which is equivalent to  $c \wedge x_1 \wedge x_2 \nleq b$ . Since *b* is a pseudo-complement of *a* in *L*,  $c \wedge x_1 \wedge x_2 \nleq b$  holds if and only if

$$a \wedge c \wedge x_1 \wedge x_2 \neq 0.$$

Now, consider the elements  $a, x_1, x_2 \in L$ .  $a \land x_1 \land x_2 \neq 0$  because otherwise we would have  $x_1 \land x_2 \leq b$ , as b is a pseudo-complement of a. Moreover  $c \wedge x_k \neq 0$  for each k, because otherwise we would have  $c \wedge x_k \leq b$ . Finally  $c \wedge a \neq 0$ , because otherwise  $c \leq b$ , contradicting our assumption. As c is a  $\mu$ -element in *L*, we conclude that  $c \wedge a \wedge x_1 \wedge x_2 \neq 0$ , which proves the claim.  $\Box$ 

**Remark 3.16.** — An analogue of part (2) of Proposition 3.15 does not hold for upsets. Consider the frame of power set  $\mathcal{P}(X)$  of the set  $X = \{1,2,3,4,5\}$ . We have  $\{1,2\} \sim_{\mathcal{U}} \{1\}^{\uparrow}$  and  $\{3,4\} \sim_{\mathcal{U}} \{3\}^{\uparrow}$ , by Remark 3.12. However, it is easy to see that  $\{1,2\} \vee \{3,4\} = \{1,2,3,4\}$  is not a  $\mu$ -element in  $\{1,3\}^{\uparrow} = \{1\} \vee \{3\}^{\uparrow}$ . Moreover, it is also not a  $\mu$ -element in  $\mathcal{P}(X)$ .

**Proposition 3.17.** — Let L be a frame,  $a \in L$ , and b a pseudo-complement of a in L. If  $c \in L$  is maximal relative to the properties  $a \leq c$  and  $b \wedge c = 0$ , then  $a \rightsquigarrow_{\mathfrak{U}} c^{\downarrow}$ .