where  $R^{\varepsilon} = R_2^{\varepsilon} + \text{div}(R_1^{\varepsilon}) + R_3^{\varepsilon} + R_4^{\varepsilon}$  and  $C_1$  is some positive constant independent of  $\varepsilon$ . Therefore,

$$\lim_{\varepsilon \to 0} \left\| \frac{G(I + \varepsilon h) - G(I)}{\varepsilon} - (\xi, \eta) \right\|_{X} = \lim_{\varepsilon \to 0} \left\| (\tilde{\xi}, \tilde{\eta}) \right\|_{X} = 0$$

This establishes the Gâteaux differentiability of G at I in the direction h, with  $G'(I)h = (\xi, \eta)$ .  $\Box$ 

Now, we establish a result on the differentiability of the cost functional:

**Theorem 4.1** (On the Gâteau-differentiability of the Cost Functional). Let Assumptions  $(A1)$ - $(A10)$  hold. Then the cost functional J is Gâteaux differentiable at any  $I \in \mathcal{U}_{ad}$ . Furthermore, for any direction  $h \in L^{\infty}(0,T)$ , the Gâteaux derivative of J at I in the direction h is given by:

$$\langle J'(I), h \rangle = \int_0^T \left[ \alpha \int_{\mathbb{R}^N} \xi(t, x) dx + 2\beta I(t) h(t) \right] dt + \gamma \int_{\mathbb{R}^N} \xi(T, x) dx \tag{45}$$

where  $(\xi,\eta)$  is the solution to the linearized system (35).

*Proof.* Let  $I \in \mathcal{U}_{ad}$  and define the functional  $L_I: L^{\infty}(0,T) \to \mathbb{R}$  by:

$$\langle L_I, h \rangle = \int_0^T \left[ \alpha \int_{\mathbb{R}^N} \xi(t, x) dx + 2\beta I(t) h(t) \right] dt + \gamma \int_{\mathbb{R}^N} \xi(T, x) dx \tag{46}$$

where  $(\xi,\eta)$  solves the linearized system (35) with the direction h. Now let  $h_1,h_2\in L^{\infty}(0,T)$  and  $\lambda \in \mathbb{R}$ , and let us consider  $h = h_1 + \lambda h_2$ , with  $(\xi_1, \eta_1)$  and  $(\xi_2, \eta_2)$  are the solutions to the linearized system corresponding to directions  $h_1$  and  $h_2$  respectively. By the linearity of system (35), the solution  $(\xi, \eta)$  corresponding to h satisfies  $\xi = \xi_1 + \lambda \xi_2$  and  $\eta = \eta_1 + \lambda \eta_2$ . Consequently:

$$\begin{split} \langle L_I, h_1 + \lambda h_2 \rangle &= \int_0^T \left[ \alpha \int_{\mathbb{R}^N} (\xi_1 + \lambda \xi_2) dx + 2\beta I(t)(h_1(t) + \lambda h_2(t)) \right] dt + \gamma \int_{\mathbb{R}^N} (\xi_1 + \lambda \xi_2)(T, x) dx \\ &= \langle L_I, h_1 \rangle + \lambda \langle L_I, h_2 \rangle. \end{split}$$

Therefore  $L_I$  is linear. Furthermore, for any  $h \in L^{\infty}(0,T)$ , by using the estimates from Lemma  $4.1$  we obtain:

$$|\langle L_I, h \rangle| \leq \alpha \int_0^T \int_{\mathbb{R}^N} |\xi(t, x)| dx dt + 2\beta \|I\|_{L^\infty} \|h\|_{L^\infty} T + \gamma \int_{\mathbb{R}^N} |\xi(T, x)| dx \leq C_1 \|h\|_{L^\infty(0, T)},$$

where  $C_1$  is a positive constant depending on  $\alpha$ ,  $\beta$ ,  $\gamma$ ,  $T$ , and the bounds from Lemma 4.1. Therefore  $L_I$  is continuous.

To show that  $L_I$  represents the Gâteaux derivative of  $J$ , let  $h \in L^{\infty}(0,T)$ ,  $\varepsilon > 0$ , and let define  $I^{\varepsilon} = I + \varepsilon h$  and let  $(p^{\varepsilon}, d^{\varepsilon}) = G(I^{\varepsilon})$  and  $(p, d) = G(I)$ . Let define  $\Phi_{I}(\varepsilon) = \frac{J(I^{\varepsilon}) - J(I)}{\varepsilon}$ , we have:

$$\begin{split} \Phi_I(\varepsilon) &= \int_0^T \left[ \alpha \int_{\mathbb{R}^N} \frac{p^\varepsilon - p}{\varepsilon} dx + \beta \frac{(I^\varepsilon)^2 - I^2}{\varepsilon} \right] dt + \gamma \int_{\mathbb{R}^N} \frac{p^\varepsilon(T, x) - p(T, x)}{\varepsilon} dx \\ &= \int_0^T \left[ \alpha \int_{\mathbb{R}^N} \xi^\varepsilon dx + \beta (2Ih + \varepsilon h^2) \right] dt + \gamma \int_{\mathbb{R}^N} \xi^\varepsilon(T, x) dx \end{split}$$

where  $\xi^{\varepsilon} = (p^{\varepsilon} - p)/\varepsilon$ . By Lemma 4.1, we have  $\xi^{\varepsilon} \to \xi$  in X as  $\varepsilon \to 0$ , where  $\xi$  is the solution to the linearized system  $(35)$ . Therefore:

$$\lim_{\varepsilon \to 0} \Phi_I(\varepsilon) = \int_0^T \left[ \alpha \int_{\mathbb{R}^N} \xi(t, x) dx + 2\beta I(t) h(t) \right] dt + \gamma \int_{\mathbb{R}^N} \xi(T, x) dx = \langle L_I, h \rangle. \tag{47}$$

This establishes that J is Gâteaux differentiable at I with derivative  $J'(I) = L_I$ , which complete the proof.  $\Box$