[{"bbox": [141, 159, 1312, 245], "category": "Text", "text": "which converges in $\\mathcal{O}_{M_{LT,\\infty}}^{L\\text{-la}}(U)$. Later we will show $D_i(s)$ actually lies in the smaller subspace $\\mathcal{O}_{M_{LT,\\infty}}^{L\\text{-la},\\mathbf{m}^0=0}(U)$.\nUsing $E_{d,i}(x_i - x_{i,n}) = 1$, a direct computation shows $E_{d,i} \\cdot D_i(s) = 0$ for all $s \\in \\mathcal{O}_{M_{LT,\\infty}}^{L\\text{-la},\\mathbf{m}^0=0}(U)$, and"}, {"bbox": [607, 261, 849, 341], "category": "Formula", "text": "$$s = \\sum_{l=0}^{\\infty} a_{i,l} (x_i - x_{i,n})^l$$"}, {"bbox": [141, 359, 1312, 456], "category": "Text", "text": "with $a_{i,l} = D_i(\\frac{(E_{d,i})^{l \\cdot s}}{l!})$. Here we note the coefficients $a_{i,l}$ are determined by $s$. From the construction we know the coefficients $a_{i,l}$ are killed by $E_{d,i}$ for all $l$. For $j \\neq i$, we further express the coefficients $a_{i,l}$ along $E_{d,j}$, namely"}, {"bbox": [576, 472, 876, 552], "category": "Formula", "text": "$$a_{i,l} = \\sum_{k=0}^{\\infty} b_{i,l,j,l'} (x_j - x_{j,n})^{l'}$$"}, {"bbox": [141, 570, 1312, 642], "category": "Text", "text": "with $b_{i,l,j,l'} = D_j(\\frac{(E_{d,j})^{l' \\cdot a_{i,l}}}{l'!})$. As $[E_{d,i}, E_{d,j}] = 0$ for $i, j = 0, 1, \\dots, d-1$, we see $b_{i,l,j,l'}$ is killed by $E_{d,i}$ and $E_{d,j}$. After we expand $s$ along each derivation $E_{d,i}$ for $i = 0, 1, \\dots, d-1$, we arrive at an expression"}, {"bbox": [377, 658, 1075, 739], "category": "Formula", "text": "$$s = \\sum_{i_0=0}^{\\infty} \\sum_{i_1=0}^{\\infty} \\cdots \\sum_{i_{d-1}=0}^{\\infty} c_{i_0 \\dots i_{d-1}} (x_0 - x_{0,n})^{i_0} \\cdots (x_{d-1} - x_{d-1,n})^{i_{d-1}}$$"}, {"bbox": [141, 757, 1312, 819], "category": "Text", "text": "such that $E_{d,i}c_{i_0 \\dots i_{d-1}} = 0$ for all $i = 0, 1, \\dots, d-1$. As $\\mathbf{m}^0$ acts trivially on $\\mathcal{O}_{\\mathcal{F}\\ell}$, we know $\\mathbf{m}^0$ acts trivially on $x_i - x_{i,n}$ for any $i = 0, \\dots, d-1$. Therefore,"}, {"bbox": [404, 838, 1045, 903], "category": "Formula", "text": "$$0 = \\sum_{i_0, \\dots, i_{d-1}} (\\mathbf{m}^0 c_{i_0 \\dots i_{d-1}}) (x_0 - x_{0,n})^{i_0} \\cdots (x_{d-1} - x_{d-1,n})^{i_{d-1}}$$"}, {"bbox": [141, 921, 1312, 1174], "category": "Text", "text": "This implies $\\mathbf{m}^0 c_{i_0 \\dots i_{d-1}} = 0$. Indeed, the coefficients $c_{i_0 \\dots i_{d-1}}$ are determined by $s$. Combined this with the fact that $\\mathcal{O}_{M_{LT,\\infty}}^{L\\text{-la}}$ is killed by $\\pi^{-1}\\mathbf{n}^0$, we see $\\mathbf{p}^0$ kills $c_{i_0 \\dots i_{d-1}}$. Hence there is an induced action of $\\bar{\\mathbf{n}}^0 = \\mathfrak{g}^0/\\mathfrak{p}^0$ on $c_{i_0 \\dots i_{d-1}}$. On $U$, $\\bar{\\mathbf{n}}^0$ is generated by $E_{d,i}$ for $i = 0, 1, \\dots, d-1$. Indeed, on the open locus $V_o = \\{[z_0 : z_1 : \\dots : z_{d-1} : 1]\\} \\subset \\mathbb{P}^d$, the matrix $Z = \\begin{pmatrix} I_{d \\times d} & 0 \\\\ (z_0, z_1, \\dots, z_{d-1}) & 1 \\end{pmatrix}$ is a lifting of the point $z = [z_0 : z_1 : \\dots : z_{d-1} : 1]$ as $oZ = z$ where $o = [0 : 0 : \\dots : 0 : 1]$. Then $Z^{-1}E_{d,i}Z = E_{d,i}$ for $i = 0, 1, \\dots, d$ generates $\\bar{\\mathbf{n}}^0$ on $V_o$. From the construction we know $c_{i_0 \\dots i_{d-1}}$ is killed by $E_{d,i}$ for all $i = 0, 1, \\dots, d-1$, hence it is killed by $\\bar{\\mathbf{n}}^0$. This shows that $\\mathfrak{g}^0$ acts trivially on $c_{i_0 \\dots i_{d-1}}$, which implies $c_{i_0 \\dots i_{d-1}} \\in \\mathcal{O}_{M_{LT,\\infty}}^{\\text{sm}}(U)$. $\\square$"}, {"bbox": [141, 1193, 1312, 1277], "category": "Text", "text": "**Corollary 0.3.2.** For any $U \\in \\mathfrak{B}_{LT}$, the image of $\\mathcal{O}_{M_{LT,\\infty}}^{\\text{sm}}(U) \\otimes_C \\pi^{-1}\\mathcal{O}_{\\mathcal{F}\\ell}(U)$ inside $\\mathcal{O}_{M_{LT,\\infty}}^{L\\text{-la},\\mathbf{m}^0=0}(U)$ is dense.\n\n*Proof.* This follows directly from Theorem 0.3.1. $\\square$"}, {"bbox": [141, 1292, 1312, 1413], "category": "Text", "text": "To simplify the notation, we denote $\\mathcal{O}_{LT}$ by the sheaf $\\mathcal{O}_{M_{LT,\\infty}}^{L\\text{-la},\\mathbf{m}^0=0}$ on $M_{LT,\\infty}$. Put $\\mathcal{O}_{LT}^{\\text{sm}} := \\mathcal{O}_{M_{LT,\\infty}}^{G\\text{-sm}}$. Let $\\Omega_{M_{LT,n}}^k$ be the sheaf of $k$-differential forms on $M_{LT,n}$ for $k = 0, 1, \\dots, d$ and put $\\Omega_{LT}^{k,\\text{sm}} := \\varinjlim_{n \\to \\infty} \\pi_n^{-1}\\Omega_{M_{LT,n}}^k$ with $\\pi_n : M_{LT,\\infty} \\to M_{LT,n}$. Clearly $\\mathcal{O}_{LT}^{\\text{sm}} = \\Omega_{LT}^{0,\\text{sm}}$ and $\\Omega_{LT}^{k,\\text{sm}} = \\wedge_{\\mathcal{O}_{LT}^{\\text{sm}}}^k \\Omega_{LT}^{1,\\text{sm}}$."}, {"bbox": [141, 1424, 1153, 1552], "category": "Text", "text": "**Proposition 0.3.3.** There exists a differential operator $d : \\mathcal{O}_{LT} \\to \\mathcal{O}_{LT} \\otimes_{\\mathcal{O}_{LT}^{\\text{sm}}} \\Omega_{LT}^{1,\\text{sm}}$, such that\n(i) $d$ is given by the usual derivation on $\\mathcal{O}_{LT}^{\\text{sm}}$,\n(ii) $d$ is $\\pi^{-1}\\mathcal{O}_{\\mathcal{F}\\ell}$-linear."}, {"bbox": [141, 1566, 961, 1597], "category": "Text", "text": "Moreover, $d$ is uniquely determined by these two properties up to constants."}, {"bbox": [141, 1610, 1312, 1703], "category": "Text", "text": "*Proof.* Define $d|_{\\mathcal{O}_{LT}^{\\text{sm}}}$ as the differential map on finite levels $\\mathcal{O}_{LT}^{\\text{sm}} \\to \\Omega_{LT}^{1,\\text{sm}}$, and define $d|_{\\pi^{-1}\\mathcal{O}_{\\mathcal{F}\\ell}}$ to be the zero map. By Theorem 0.3.1, for any $U \\in \\mathfrak{B}_{LT}$ such that $z_d \\neq 0$ on $U$, we may write any section $s \\in \\mathcal{O}_{LT}(U)$ of the form for some sufficiently large $n$:"}, {"bbox": [377, 1717, 1075, 1799], "category": "Formula", "text": "$$s = \\sum_{i_0=0}^{\\infty} \\sum_{i_1=0}^{\\infty} \\cdots \\sum_{i_{d-1}=0}^{\\infty} c_{i_0 \\dots i_{d-1}} (x_0 - x_{0,n})^{i_0} \\cdots (x_{d-1} - x_{d-1,n})^{i_{d-1}}$$"}]