[{"bbox": [208, 275, 1359, 345], "category": "Text", "text": "**Theorem 3.6.** Let $\\mathbf{x} \\preceq (0, \\dots, n-1)$ be an irreducible score, so that $C \\cap (0, \\infty)^{n \\times n} \\neq \\emptyset$. Then"}, {"bbox": [447, 349, 1357, 404], "category": "Formula", "text": "$$ \\lim_{k \\to \\infty} M^k = \\arg \\min_{L \\in C} D(L, M^0) = \\arg \\min_{L \\in C} H(L). \\quad (3.9) $$"}, {"bbox": [208, 427, 1343, 465], "category": "Text", "text": "*Proof.* Note that $\\text{dom}(h) = \\mathbb{R}_+$, $\\text{idom}(h) = (0, \\infty)$ and $\\text{bdom}(h) = \\{0\\}$. It is easy to check:"}, {"bbox": [255, 477, 1357, 792], "category": "List-item", "text": "(1) $h$ is a proper convex function. Moreover, $h$ is closed because $\\{x \\in \\text{dom}(h) : h(x) \\le \\alpha\\}$ is closed for all $\\alpha \\in \\mathbb{R}$.\n(2) $h$ is Legendre because\n• $h$ is differentiable on $\\text{idom}(h)$;\n• $\\lim_{t \\to 0+} h'(x + t(y - x))(y - x) = -\\infty$ for all $x \\in \\text{bdom}(f)$ and $y \\in \\text{idom}(h)$;\n• $h$ is strictly convex on $\\text{idom}(h)$.\n(3) $h$ is co-finite because $\\lim_{t \\to \\infty} \\frac{h(tx)}{t} = \\infty$ for all $x \\neq 0$.\n(4) $h$ is very strictly convex because $h''(x) > 0$ for all $x \\in \\text{idom}(h)$."}, {"bbox": [208, 803, 1292, 839], "category": "Text", "text": "Since $C_1, C_2, C_3$ are all affine subsets, it suffices to apply [7, Theorem 4.3] to conclude. $\\square$"}, {"bbox": [208, 868, 1359, 937], "category": "Text", "text": "See also [45] for recent development on the convergence rate of Bregman's iteration under further technical assumptions, which we do not pursue here."}, {"bbox": [208, 941, 1359, 1040], "category": "Text", "text": "Next we propose a computational scheme inspired by Theorem 3.6. The key is to compute numerically, for each $M \\in (0, \\infty)^{n \\times n}$, its Bregman projection on $C_k$. We distinguish three cases:"}, {"bbox": [277, 1054, 1359, 1210], "category": "List-item", "text": "• $k=1$: We introduce the Lagrange multiplier $\\lambda = (\\lambda_1, \\dots, \\lambda_n) \\in \\mathbb{R}^n$, and set $\\Phi(L, \\lambda) := D(L, M) + \\sum_{i=1}^n \\lambda_i (\\sum_{j=1}^n l_{ij} - 1)$. Differentiating $\\Phi$ with respect to $m_{ij}$ and $\\lambda_i$ yields $\\partial_{l_{ij}} \\Phi = \\log(l_{ij}) - \\log(m_{ij}) + \\lambda_i$ and $\\partial_{\\lambda_i} \\Phi = \\sum_{j=1}^n l_{ij} - 1$. By setting these to zero, we get"}, {"bbox": [497, 1223, 1357, 1306], "category": "Formula", "text": "$$ \\arg \\min_{L \\in C_1} D(L, M) = \\left( \\frac{m_{ij}}{\\sum_{k=1}^{n} m_{ik}} \\right)_{1 \\le i, j \\le n}. \\quad (3.10) $$"}, {"bbox": [277, 1318, 1025, 1353], "category": "List-item", "text": "• $k=2$: The same reasoning as in the previous case yields:"}, {"bbox": [497, 1366, 1357, 1448], "category": "Formula", "text": "$$ \\arg \\min_{L \\in C_2} D(L, M) = \\left( \\frac{m_{ij}}{\\sum_{k=1}^{n} m_{kj}} \\right)_{1 \\le i, j \\le n}. \\quad (3.11) $$"}, {"bbox": [277, 1463, 1359, 1593], "category": "List-item", "text": "• $k=3$: Define $\\Phi(L, \\lambda) := D(L, M) + \\sum_{i=1}^n \\lambda_i (\\sum_{j=1}^n (j-1)l_{ij} - x_i)$, and differentiate $\\Phi$ with respect to $m_{ij}$ and $\\lambda_i$ yields $\\partial_{l_{ij}} \\Phi = \\log(l_{ij}) - \\log(m_{ij}) + \\lambda_i(j-1)$ and $\\partial_{\\lambda_i} \\Phi = \\sum_{j=1}^n (j-1)l_{ij} - x_i$. Setting these to zero yields"}, {"bbox": [517, 1606, 1357, 1671], "category": "Formula", "text": "$$ \\arg \\min_{L \\in C_3} D(L, M) = (m_{ij} r_{ij}^{j-1})_{1 \\le i, j \\le n}, \\quad (3.12) $$"}, {"bbox": [304, 1684, 1359, 1831], "category": "Text", "text": "where $r_{ij}$ is the unique positive root to the polynomial equation $\\sum_{j=1}^n (j-1)m_{ij}r_{ij}^{j-1} - x_i = 0$. Let $f(r) := \\sum_{j=1}^n (j-1)m_{ij}r_{ij}^{j-1} - x_i$. It is easy to see that $f$ is strictly increasing on $[0, \\infty)$ with $f(0) \\le 0$ and $\\lim_{r \\to \\infty} f(r) = +\\infty$. Thus, it is easy (and quick) to find a numerical root of $f$ on $[0, \\infty)$ by Newton's method."}]