[{"bbox": [346, 193, 1195, 218], "category": "Page-header", "text": "14 GERALD ALSMEYER, KONRAD KOLESKO, MATTHIAS MEINERS, AND JAKOB STONNER"}, {"bbox": [259, 244, 1044, 282], "category": "Text", "text": "Define $a_0 := \\infty$, $a_n := \\sum_{k \\ge n} \\mu_+^{-1}(\\delta^k)/k$ for $n \\in \\mathbb{N}$, and the function $\\psi$ by"}, {"bbox": [568, 296, 971, 357], "category": "Formula", "text": "$$ \\psi(t) := \\sum_{n \\in \\mathbb{N}_0} \\delta^n \\mathbb{1}_{(a_{n+1}, a_n]}(t), \\quad t \\ge 0. $$"}, {"bbox": [261, 369, 319, 397], "category": "Text", "text": "Then"}, {"bbox": [505, 393, 1037, 456], "category": "Formula", "text": "$$ F(t) \\le \\psi(4t) \\quad \\text{for all } t \\le t_0 := \\frac{\\delta}{4(2+\\delta)} \\mu_+^{-1}(1). $$"}, {"bbox": [259, 469, 1283, 587], "category": "Text", "text": "**Proof.** The assumptions imply that $\\mu_+$ is continuous and strictly increasing and hence is the cumulative mass function of a continuous measure on $[0, \\infty)$. Moreover, $\\mu_+$ is a bijection of $[0, \\infty)$, and its generalized inverse $\\mu_+^{-1}$ is simply the inverse function. Let $\\psi_0 = \\psi$, and for $n \\in \\mathbb{N}$, define $\\psi_n$ recursively by"}, {"bbox": [410, 598, 1131, 667], "category": "Formula", "text": "$$ \\psi_{n+1}(t) := 1 - \\exp \\left( - \\psi_n(t) - \\int_0^{t/4} \\psi_n(t-4x) \\mu_+(dx) \\right), \\quad t \\ge 0. $$"}, {"bbox": [259, 676, 1283, 762], "category": "Text", "text": "Denote by $\\mathbf{T}$ denoting the smoothing transform associated with the Poisson point process with intensity measure $\\mu = \\delta_0 + \\mu_+$ as given by (3.2) and its representation (5.1). By induction, we observe that"}, {"bbox": [541, 765, 1001, 800], "category": "Formula", "text": "$$ 1 - \\psi_n(4t) = \\mathbf{T}^n [1 - \\psi(4\\cdot)](t), \\quad t \\ge 0. $$"}, {"bbox": [259, 807, 1099, 837], "category": "Text", "text": "Thus, by Theorem 3.4(b), we infer that $\\psi_n(4t) \\to F(t)$ as $n \\to \\infty$ for all $t > 0$."}, {"bbox": [259, 843, 1283, 930], "category": "Text", "text": "To complete the proof, it remains to show that $\\psi_n(t) \\le \\psi(t)$ holds for all $t \\le 4t_0$ and $n \\in \\mathbb{N}_0$. We will prove the slightly stronger statement $\\psi_n(t) \\le \\psi(t)$ for all $t \\le a_{k_0}$ via induction on $n$, where $k_0 \\in \\mathbb{N}_0$ is chosen such that"}, {"bbox": [662, 946, 1283, 976], "category": "Formula", "text": "$$ a_{k_0+1} < 4t_0 \\le a_{k_0}. \\qquad (5.3) $$"}, {"bbox": [259, 989, 1283, 1107], "category": "Text", "text": "For $n=0$, the claim is trivially true (base case). For the inductive step, assume $\\psi_n(t) \\le \\psi(t)$ for all $t \\le a_{k_0}$ and some $n \\in \\mathbb{N}_0$. We will show that $\\psi_{n+1}(t) \\le \\psi(t)$ for all $t \\in (a_{k_1}, a_k]$ and $k \\ge k_0$. If $k_0 = 0$, for $t > a_1$ we clearly have $\\psi(t) = 1 \\ge \\psi_{n+1}(t)$. Thus we can assume $k \\ge k_0 \\lor 1$. Let $t \\in (a_{k_1}, a_k]$ for $k \\ge k_0 \\lor 1$. Then we have"}, {"bbox": [365, 1119, 1172, 1299], "category": "Formula", "text": "$$ \\begin{align*} \\psi_{n+1}(t) \\le \\psi_{n+1}(a_k) &= 1 - \\exp \\left( -\\psi_n(a_k) - \\int_0^{a_k/4} \\psi_n(a_k - 4x) \\mu_+(dx) \\right) \\\\ &\\le 1 - \\exp \\left( -\\psi(a_k) - \\int_0^{a_k/4} \\psi(a_k - 4x) \\mu_+(dx) \\right) \\\\ &= 1 - \\exp \\left( -(\\psi(t) + I_k) \\right) \\end{align*} $$"}, {"bbox": [259, 1310, 1151, 1339], "category": "Text", "text": "where $I_k$ represents the integral in the exponent. To estimate $I_k$, we first note that"}, {"bbox": [365, 1350, 1175, 1677], "category": "Formula", "text": "$$ \\begin{align*} I_k &= \\int_0^{a_k/4} \\psi(a_k - 4x) \\mu_+(dx) = \\sum_{j \\ge k} \\int_{[a_k - a_j, a_k - a_{j+1})/4} \\psi(a_k - 4x) \\mu_+(dx) \\\\ &= \\sum_{j \\ge k} \\delta^j \\left[ \\mu_+\\left(\\frac{a_k - a_{j+1}}{4}\\right) - \\mu_+\\left(\\frac{a_k - a_j}{4}\\right) \\right] \\\\ &= \\delta^k \\sum_{j=0}^{\\infty} \\delta^j \\left[ \\mu_+\\left(\\frac{a_k - a_{k+j+1}}{4}\\right) - \\mu_+\\left(\\frac{a_k - a_{k+j}}{4}\\right) \\right] \\\\ &= \\psi(t) \\sum_{j=0}^{\\infty} \\delta^j (1 - \\delta) \\mu_+\\left(\\frac{a_k - a_{k+j+1}}{4}\\right), \\end{align*} $$"}]