and then observing that the canonical function of $Y$ writes as $k ( x ) = \lambda e ^ { A x - B | x | }$ , implying $\tau _ { + } ^ { - A } = \tau _ { - } ^ { A } = \lambda \delta _ { B }$ . The Dirac integration to which (5.25) reduces, produces  

$$
k _ { \rho } ( x ) = \lambda e ^ { ( A ^ { 2 } - B ^ { 2 } ) x / 2 } = \lambda e ^ { - \theta _ { + } \theta _ { - } x / 2 } .
$$  

Therefore, the bilateral gamma process can be represented in law as $Y _ { t } = W _ { T _ { t } } + ( \theta _ { - } - \theta _ { + } ) t / 2$ where $\mathscr { L } ( T _ { 1 } ) \sim \Gamma ( \lambda , \theta _ { + } \theta _ { - } / 2 )$ . This has been known and used at least since Madan et al. (1998).  

Example 10. Subordinated representation of CTS $\alpha$ processes. Madan and Yor (2008) through a series of propositions covering a substantial part of the article, explain how to represent a $\mathrm { C T S } _ { \alpha } ( \mathbb { R } )$ process as a subordinated Brownian motion with drift. Based on the discussion so far, the main Proposition 2 therein trivialize. First of all notice that the assumptions in Theorem 6 are met also in the case of CTS $\mathbf { \alpha } _ { \alpha } ( \mathbb { R } )$ processes with symmetric spherical part. Namely, assuming $\lambda _ { + } = \lambda _ { - }$ and letting again $A = ( \theta _ { - } - \theta _ { + } ) / 2$ , $B = ( \theta _ { - } + \theta _ { - } ) / 2$ , leads to $k ( x ) =$ $x ^ { - \alpha } e ^ { A x - B | x | }$ , so that using the Thorin measure found in Subsection 4.3 we deduce the required density relationship $\tau _ { + } ^ { - A } ( y ) ~ = ~ \tau _ { - } ^ { A } ( y ) ~ = ~ \lambda ( y - B ) ^ { \alpha - 1 } ( \Gamma ( \alpha ) ) ^ { - 1 } \mathbb { 1 } _ { \{ y \geq B \} }$ . It then follows from Corollary 6, and with the substitution $w = ( s - B ) \sqrt { x }$ , that  

$$
\begin{array} { l } { { k _ { \rho } ( x ) = \lambda \displaystyle \frac { e ^ { x A ^ { 2 } / 2 } } { \Gamma ( \alpha ) } \int _ { B } ^ { \infty } e ^ { - \frac { s ^ { 2 } x } { 2 } } ( s - B ) ^ { \alpha - 1 } d s = \lambda \displaystyle \frac { e ^ { ( A ^ { 2 } - B ^ { 2 } ) x / 2 } } { \Gamma ( \alpha ) x ^ { \alpha / 2 } } \int _ { 0 } ^ { \infty } e ^ { - \frac { w ^ { 2 } } { 2 } - w B \sqrt { x } } w ^ { \alpha - 1 } d w } } \\ { { = \lambda \displaystyle \frac { e ^ { - \theta _ { + } \theta _ { - } x / 2 } } { x ^ { \alpha / 2 } } H _ { - \alpha } \left( \frac { \theta _ { + } + \theta _ { - } } { 2 } \sqrt { x } \right) } } \end{array}
$$  

where $H _ { a }$ , $a < 0$ , is the Hermite function, given by  

$$
H _ { a } ( z ) = \frac { 1 } { \Gamma ( - a ) } \int _ { 0 } ^ { \infty } e ^ { - x ^ { 2 } / 2 - x z } x ^ { - a - 1 } d x , \qquad z > 0 .
$$  

The corresponding Le´vy density coincides with that determined in Madan and Yor (2008), Proposition 2.  

Example 11. Subordinated representation of generalized- $z$ processes. Let $\mu \in \operatorname { G Z D } _ { G } ( \mathbb { R } )$ with Le´vy measure of the form (4.20), i.e. $c ( \pm 1 ) = c _ { \pm } > 0$ , $\sigma ( \pm ) = \sigma > 0$ and $\lambda ( d u ) = \lambda ( \delta _ { 1 } ( d u ) +$ $\delta _ { - 1 } ( d u ) )$ , $\lambda > 0$ . We can rewrite again $k ( x ) = e ^ { A x / \sigma - B | x | / \sigma } / ( 1 - e ^ { - | x | / \sigma } )$ , $A = ( c _ { - } - c _ { + } ) / 2$ , $B = ( c _ { - } + c _ { + } ) / 2$ so we are under the assumption of Theorem 6. Based on (4.22) and (5.25), integrating term by term the series results in  

$$
\begin{array} { l } { { \displaystyle k _ { \rho } ( x ) = \lambda e ^ { \frac { A ^ { 2 } x } { 2 \sigma ^ { 2 } } } \sum _ { k = 0 } ^ { \infty } \exp \left( - x \frac { ( k + B ) ^ { 2 } } { 2 \sigma ^ { 2 } } \right) = \lambda \sum _ { k = 0 } ^ { \infty } \exp \left( - x \frac { k ^ { 2 } + 2 B k + B ^ { 2 } - A ^ { 2 } } { 2 \sigma ^ { 2 } } \right) } } \\ { { \displaystyle ~ = \lambda \sum _ { k = 0 } ^ { \infty } \exp \left( - x \frac { ( k + c _ { + } ) ( k + c _ { - } ) } { 2 \sigma ^ { 2 } } \right) . } } \end{array}
$$  

The subordinator is then of the form of an infinite GGC convolution of gamma processes $G ^ { k } = ( G _ { t } ^ { k } ) _ { t \geq 0 }$ , $k \geq 0$ , $\begin{array} { r } { \mathcal { L } ( G _ { 1 } ^ { k } ) \sim \Gamma \left( \lambda , \frac { ( k + c _ { + } ) ( k + c _ { - } ) } { 2 \sigma ^ { 2 } } \right) } \end{array}$ whose limit in law is not otherwise known.  