Notice that $n _ { i } = n _ { i } ^ { 1 } \wedge n _ { i } ^ { 2 }$ . Thus,  

$$
\bigwedge _ { i = 1 } ^ { 2 } n _ { i } = \bigwedge _ { i = 1 } ^ { 2 } ( n _ { i } ^ { 1 } \wedge n _ { i } ^ { 2 } ) .
$$  

Since $( a _ { 1 } \land a _ { 2 } ) \land n _ { i } \neq 0$ for each $i$ , we get  

$$
0 \neq { \big ( } a _ { 1 } \wedge a _ { 2 } { \big ) } \wedge n _ { i } = { \big ( } a _ { 1 } \wedge a _ { 2 } { \big ) } \wedge { \big ( } n _ { i } ^ { 1 } \wedge n _ { i } ^ { 2 } { \big ) } = { \big ( } a _ { 1 } \wedge n _ { i } ^ { 1 } { \big ) } \wedge { \big ( } a _ { 2 } \wedge n _ { i } ^ { 2 } { \big ) } .
$$  

This implies that $a _ { 1 } \wedge n _ { i } ^ { 1 } \neq 0$ and $a _ { 2 } \wedge n _ { i } ^ { 2 } \not = 0$ . Since $a _ { 1 } \gamma _ { \mu } b _ { 1 } ^ { \dagger }$ and $a _ { 2 } \gamma _ { \mu } b _ { 2 } ^ { \dagger }$ , we have  

$$
a _ { 1 } \wedge \left( \bigwedge _ { i = 1 } ^ { 2 } n _ { i } ^ { 1 } \right) \neq 0 \quad \mathrm { a n d } \quad a _ { 2 } \wedge \left( \bigwedge _ { i = 1 } ^ { 2 } n _ { i } ^ { 2 } \right) \neq 0 .
$$  

Thus,  

$$
\big ( a _ { 1 } \wedge a _ { 2 } \big ) \wedge \left( \bigwedge _ { i = 1 } ^ { 2 } n _ { i } \right) = \big ( a _ { 1 } \wedge a _ { 2 } \big ) \wedge \left( \bigwedge _ { i = 1 } ^ { 2 } ( n _ { i } ^ { 1 } \wedge n _ { i } ^ { 2 } ) \right) \neq 0 .
$$  

Therefore, $( a _ { 1 } \wedge a _ { 2 } ) \sim _ { \mu } ( b _ { 1 } \wedge b _ { 2 } ) ^ { \downarrow }$ .  

(3) Let $x _ { 1 }$ and $x _ { 2 }$ be nonzero elements in $b ^ { \downarrow }$ such that $x _ { 1 } \wedge x _ { 2 } \neq 0$ and $( a \wedge b ) \wedge x _ { k } \neq 0$ for each $k$ . This implies $a \wedge ( b \wedge x _ { k } ) \neq 0$ for each $k$ . Also, observe that $\textstyle \bigwedge _ { k = 1 } ^ { 2 } \left( b \wedge x _ { k } \right) = b \wedge \left( x _ { 1 } \wedge x _ { 2 } \right) = x _ { 1 } \wedge x _ { 2 } \neq 0$ . Since $a$ is a $\mu$ -element in $L$ , this implies that  

$$
\bigl ( a \wedge b \bigr ) \wedge \bigl ( x _ { 1 } \wedge x _ { 2 } \bigr ) = a \wedge \left( \bigwedge _ { k = 1 } ^ { 2 } \bigl ( b \wedge x _ { k } \bigr ) \right) \neq 0 ,
$$  

proving the desired claim.  

(4) We can assume $a \neq 0$ and $a \neq 1$ , because otherwise $b = 1$ or $b = 0$ respectively, and the thesis holds. We can also assume that $c \notin b$ , because otherwise $b \vee c = b \ightsquigarrow _ { \mu } b ^ { \uparrow }$ . Let $x _ { 1 } > b$ and $x _ { 2 } > b$ such that $\left( x _ { 1 } \wedge x _ { 2 } \right) > b$ and $( ( b \lor c ) \land x _ { k } ) > b$ , for each $k$ . The latter condition is equivalent to $b \vee \left( c \wedge x _ { k } \right) > b$ , which is equivalent to $c \land x _ { k } \nless b$ . We need to show that  

$$
( b \lor c ) \land x _ { 1 } \land x _ { 2 } > b ,
$$  

which is equivalent to $c \land x _ { 1 } \land x _ { 2 } \nmid k$ . Since $b$ is a pseudo-complement of $a$ in L $, c \wedge x _ { 1 } \wedge x _ { 2 } \not \in b$ holds if and only if  

$$
a \wedge c \wedge x _ { 1 } \wedge x _ { 2 } \neq 0 .
$$  

Now, consider the elements $a , x _ { 1 } , x _ { 2 } \in L$ . $a \wedge x _ { 1 } \wedge x _ { 2 } \neq 0$ because otherwise we would have $x _ { 1 } \land x _ { 2 } \leqslant b$ , as $b$ is a pseudo-complement of $a$ . Moreover $c \wedge x _ { k } \neq 0$ for each $k$ , because otherwise we would have $c \land x _ { k } \leqslant b$ . Finally $c \wedge a \not = 0$ , because otherwise $c \leqslant b$ , contradicting our assumption. As $c$ is a $\mu$ -element in $L$ , we conclude that $c \wedge a \wedge x _ { 1 } \wedge x _ { 2 } \neq 0$ , which proves the claim. □  

Remark 3.16. — An analogue of part (2) of Proposition 3.15 does not hold for upsets. Consider the frame of power set ${ \mathcal { P } } ( X )$ of the set $X = \{ 1 , 2 , 3 , 4 , 5 \}$ . We have $\{ 1 , 2 \} \sim _ { \mu } \{ 1 \} ^ { \uparrow }$ and $\{ 3 , 4 \} \sim _ { \mu } \{ 3 \} ^ { \uparrow }$ , by Remark 3.12. However, it is easy to see that $\{ 1 , 2 \} \vee \{ 3 , 4 \} = \{ 1 , 2 , 3 , 4 \}$ is not a $\mu$ -element in $\{ 1 , 3 \} ^ { \uparrow } = \{ 1 \} \vee \{ 3 \} ^ { \uparrow }$ . Moreover, it is also not a $\mu$ -element in ${ \mathcal { P } } ( X )$ .  

Proposition 3.17. — Let L be a frame, $a \in L ,$ and $b$ a pseudo-complement of a in $L .$ If $c \in L$ is maximal relative to the properties $a \leqslant c$ and $b \wedge c = 0$ , then $a \sim _ { \mu } c ^ { \downarrow }$ .  