Theorem 3.6. Let $\mathbf { x } \preceq ( 0 , \ldots , n - 1 )$ be an irreducible score, so that $C \cap ( 0 , \infty ) ^ { n \times n } \neq \emptyset$ Then  

$$
\operatorname* { l i m } _ { k \to \infty } { M ^ { k } } = \arg \operatorname* { m i n } _ { L \in { \cal C } } D ( L , { M ^ { 0 } } ) = \arg \operatorname* { m i n } _ { L \in { \cal C } } H ( L ) .
$$  

Proof. Note that $\mathrm { d o m } ( h ) = \mathbb { R } _ { + }$ , $\mathrm { i d o m } ( h ) = ( 0 , \infty )$ and $\mathrm { b d o m } ( h ) = \{ 0 \}$ . It is easy to check:  

(1) $h$ is a proper convex function. Moreover, $h$ is closed because $\{ x \in \operatorname { d o m } ( h ) : h ( x ) \leq \alpha \}$ is closed for all $\alpha \in \mathbb { R }$ .  

(2) $h$ is Legendre because  

• $h$ is differentiable on $\operatorname { i d o m } ( h )$ ;   
• $\begin{array} { r } { \operatorname* { l i m } _ { t  0 + } h ^ { \prime } ( x + t ( y - x ) ) ( y - x ) = - \infty } \end{array}$ for all $x \in \operatorname { b d o m } ( f )$ and $y \in \operatorname { i d o m } ( h )$ ;   
• $h$ is strictly convex on $\operatorname { i d o m } ( h )$ . (3) $h$ is co-finite because $\begin{array} { r } { \operatorname* { l i m } _ { t  \infty } \frac { h ( t x ) } { t } = \infty } \end{array}$ for all $x \neq 0$ .   
(4) $h$ is very strictly convex because $h ^ { \prime \prime } ( x ) > 0$ for all $x \in \operatorname { i d o m } ( h )$ .  

Since $C _ { 1 } , C _ { 2 } , C _ { 3 }$ are all affine subsets, it suffices to apply [7, Theorem 4.3] to conclude.  

See also [45] for recent development on the convergence rate of Bregman’s iteration under further technical assumptions, which we do not pursue here.  

Next we propose a computational scheme inspired by Theorem 3.6. The key is to compute numerically, for each $M \in ( 0 , \infty ) ^ { n \times n }$ , its Bregman projection on $C _ { k }$ . We distinguish three cases:  

• $k ~ = ~ 1$ : We introduce the Lagrange multiplier $\lambda = ( \lambda _ { 1 } , \ldots , \lambda _ { n } ) \in \mathbb { R } ^ { n }$ , and set $\begin{array} { r } { \Phi ( L , \lambda ) : = D ( L , M ) + \sum _ { i = 1 } ^ { n } \lambda _ { i } \left( \sum _ { j = 1 } ^ { n } l _ { i j } - 1 \right) } \end{array}$ . Differentiating $\Phi$ with respect to $m _ { i j }$ and $\lambda _ { i }$ yields $\partial _ { l _ { i j } } \Phi = \log ( l _ { i j } ) - \log ( m _ { i j } ) + \lambda _ { i }$ and $\begin{array} { r } { \partial _ { \lambda _ { i } } \Phi = \sum _ { j = 1 } ^ { n } l _ { i j } - 1 } \end{array}$ . By setting these to zero, we get  

$$
\arg \operatorname* { m i n } _ { L \in { \cal C } _ { 1 } } D ( L , M ) = \left( \frac { m _ { i j } } { \sum _ { k = 1 } ^ { n } m _ { i k } } \right) _ { 1 \leq i , j \leq n } .
$$  

• $k = 2$ : The same reasoning as in the previous case yields:  

$$
\operatorname { a r g m i n } _ { L \in C _ { 2 } } D ( L , M ) = \left( \frac { m _ { i j } } { \sum _ { k = 1 } ^ { n } m _ { k j } } \right) _ { 1 \leq i , j \leq n } .
$$  

• $k = 3$ : Define $\begin{array} { r } { \Phi ( L , \lambda ) : = D ( L , M ) + \sum _ { i = 1 } ^ { n } \lambda _ { i } \left( \sum _ { j = 1 } ^ { n } ( j - 1 ) l _ { i j } - x _ { i } \right) } \end{array}$ , and differentiate $\Phi$ with respect to $m _ { i j }$ and $\lambda _ { i }$ yields $\partial _ { l _ { i j } } \Phi = \log ( l _ { i j } ) - \log ( m _ { i j } ) + \lambda _ { i } ( j - 1 )$ and $\begin{array} { r } { \partial _ { \lambda _ { i } } \Phi = \sum _ { j = 1 } ^ { n } ( j - 1 ) l _ { i j } - x _ { i } } \end{array}$ . Setting these to zero yields  

$$
\begin{array} { r } { \arg \operatorname* { m i n } _ { L \in C _ { 3 } } D ( L , M ) = \left( m _ { i j } r _ { i j } ^ { j - 1 } \right) _ { 1 \leq i , j \leq n } , } \end{array}
$$  

where $r _ { i j }$ is the unique positive root to the polynomial equation $\begin{array} { r } { \sum _ { j = 1 } ^ { n } ( j - 1 ) m _ { i j } r ^ { j - 1 } - } \end{array}$ $x _ { i } = 0$ . Let $\begin{array} { r } { f ( r ) : = \sum _ { j = 1 } ^ { n } ( j - 1 ) m _ { i j } r ^ { j - 1 } - x _ { i } } \end{array}$ . It is easy to sPee that $f$ is strictly increasing on $[ 0 , \infty )$ with $f ( 0 ) \leq 0$ and $\begin{array} { r } { \operatorname* { l i m } _ { r \to \infty } f ( r ) = + \infty } \end{array}$ . Thus, it is easy (and quick) to find a numerical root of $f$ on $[ 0 , \infty )$ by Newton’s method.  